Final MergeSort

MergeSort.dfy
@@ -9,20 +9,207 @@ predicate SortedSequence(q: seq<int>)
 	forall i,j :: 0 <= i <= j < |q| ==> q[i] <= q[j]
 }
 
-predicate isLeftArr(a: array<int>, left: array<int>, middle: nat)
-	reads left, a
+predicate isValidIndex (a: array<int>, i: nat) 
 {
-	a.Length >= 2 && middle == (a.Length - 1) / 2 && 0 < middle < a.Length &&
-	left.Length == middle + 1 &&
-	forall j :: 0 <= j < left.Length ==> left[j] == a[j]
+    0 <= i < a.Length
 }
 
-predicate isRightArr(a: array<int>, right: array<int>, middle: nat)
+method MergeSort(a: array<int>) returns (b: array<int>)
+	ensures b.Length == a.Length && Sorted(b) && multiset(a[..]) == multiset(b[..])
+	decreases a.Length, 4
+{
+    // Alternation
+    if (a.Length < 2) {
+			b := Assign1(a);
+		} else {
+			b := MergeSort1(a);
+		}
+}
+
+method Assign1 (a: array<int>) returns (b: array<int>)
+	requires a.Length < 2 // If test
+	ensures b.Length == a.Length && Sorted(b) && multiset(a[..]) == multiset(b[..])
+{
+    // Assignment
+	LemmaS1(a);
+	b := a;
+}
+
+lemma LemmaS1 (a: array<int>) 
+	requires a.Length < 2
+	ensures a.Length == a.Length && Sorted(a) && multiset(a[..]) == multiset(a[..])
+{}
+
+method MergeSort1 (a: array<int>) returns (b: array<int>)
+	requires a.Length >= 2 // !(If test)
+	ensures b.Length == a.Length && Sorted(b) && multiset(a[..]) == multiset(b[..])
+	decreases a.Length, 3
+{
+	// Sequential Composition
+	var middle := AssignMiddle(a);
+	b := MergeSort2(a, middle);
+
+}
+
+method AssignMiddle (a: array<int>) returns (m: nat) 
+	requires a.Length >= 2
+	ensures m == (a.Length - 1) / 2 && isValidIndex(a, m)
+{
+    // Assignment
+	LemmaS2(a);
+	m := (a.Length - 1) / 2;
+}
+
+lemma LemmaS2 (a: array<int>) 
+	requires a.Length >= 2
+	ensures (a.Length - 1) / 2 == (a.Length - 1) / 2 && isValidIndex(a, (a.Length - 1) / 2)
+{}
+
+method MergeSort2 (a: array<int>, middle: nat) returns (b: array<int>) 
+	requires a.Length >= 2
+	requires middle == (a.Length - 1) / 2 && isValidIndex(a, middle)
+	ensures b.Length == a.Length && Sorted(b) && multiset(a[..]) == multiset(b[..])
+	decreases a.Length, 2
+{
+	// Sequential Composition
+	var left, right, i1, i2 := Assign3Split(a, middle);
+	b := MergeSort3(a, left, right, middle, i1, i2);
+}
+
+method Assign3Split (a: array<int>, middle: nat) returns (left: array<int>, right: array<int>, i1: nat, i2: nat)
+	requires a.Length >= 2 && middle == (a.Length - 1) / 2 && isValidIndex(a, middle)
+	ensures isLeftArr(a, left, middle, i1)
+	ensures isRightArr(a, right, middle, i2)
+	ensures left.Length + right.Length == a.Length
+{
+    // Sequential Composition
+	left, i1 := Assign3Left(a, middle);
+	assert isLeftArr(a, left, middle, i1) ==> forall j :: 0 <= j < left.Length ==> left[j] == a[j];
+	right, i2 :=  Assign3Right(a, middle);
+	assert isRightArr(a, right, middle, i2) ==> forall j :: 0 <= j < right.Length ==> right[j] == a[j + middle + 1];
+
+}
+
+method Assign3Left(a: array<int>, middle: nat) returns (arr: array<int>, i: nat) 
+	requires a.Length >= 2 && middle == (a.Length - 1) / 2 && isValidIndex(a, middle) 
+	ensures isLeftArr(a, arr, middle, i) && arr.Length == middle + 1
+{
+	i, arr := 0, new int[middle+1];
+	// Iteration
+	while (i != arr.Length) 
+		decreases arr.Length - i
+		invariant Inv1(a, arr, i)
+	{
+		ghost var V0 := middle + 1 - i;
+		// Following Assignment
+		LeftLoopBody(arr, a, i, middle); 
+		assert 0 <= arr.Length - i - 1 < V0;
+		i := i+1;
+		assert 0 <= arr.Length - i < V0;
+	}
+} 
+
+predicate Inv1(a: array<int>, arr: array<int>, i: nat)
+	reads a, arr
+{
+	i <= arr.Length && isValidIndex(a, i) &&
+	forall j :: 0 <= j < i  ==> arr[j] == a[j]
+}
+
+predicate isLeftArr(a: array<int>, left: array<int>, middle: nat, i: nat)
+	reads left, a
+{
+	 i == left.Length && Inv1(a, left, i) 
+}
+
+predicate isRightArr(a: array<int>, right: array<int>, middle: nat, i: nat)
 	reads right, a
 {
-	a.Length >= 2 && middle == (a.Length - 1) / 2 && 0 < middle < a.Length &&
-	right.Length == a.Length - (middle + 1) &&
-	forall j :: 0 <= j < right.Length  ==> right[j] == a[j + (middle + 1)]
+	i == right.Length && Inv2(a, right, middle, i)
+}
+
+method LeftLoopBody(arr: array<int>, a: array<int>, i: nat, middle: nat) 
+	requires a.Length >= 2 && middle == (a.Length - 1) / 2 && isValidIndex(a, middle) 
+	requires i < arr.Length == middle + 1
+	requires Inv1(a, arr, i)
+	ensures Inv1(a, arr, i+1)
+	modifies arr
+{
+	// Assignment
+	LemmaArrI(arr, a, i, middle);
+	arr[i] := a[i];
+} 
+
+lemma LemmaArrI(arr: array<int>, a: array<int>, i: nat, middle: nat)
+	requires a.Length >= 2 && middle == (a.Length - 1) / 2 && i < arr.Length == middle + 1 && isValidIndex(a, middle) 
+	requires Inv1(a, arr, i)
+	ensures a[..i] + [a[i]] == a[..i+1]
+{}
+
+method Assign3Right(a: array<int>, middle: nat) returns (arr: array<int>, i: nat) 
+	requires a.Length >= 2 && middle == (a.Length - 1) / 2 && isValidIndex(a, middle) 
+	ensures isRightArr(a, arr, middle, i) && arr.Length == a.Length - (middle + 1)
+{
+	i, arr := 0, new int[a.Length - (middle + 1)];
+	// Iteration
+	while (i != arr.Length)
+		decreases arr.Length - i
+		invariant Inv2(a, arr, middle, i)
+	{
+		ghost var V0 := middle + 1 - i;
+		// Following Assignment
+		RightLoopBody(arr, a, i, middle); 
+		assert 0 <= arr.Length - i - 1 < V0;
+		i := i+1;
+		assert 0 <= arr.Length - i < V0;
+	}
+} 
+
+predicate Inv2(a: array<int>, arr: array<int>, middle: nat, i: nat)
+	reads a, arr
+{
+	i <= arr.Length == a.Length - (middle + 1) && isValidIndex(a, i) &&
+	forall j :: 0 <= j < i ==> arr[j] == a[j + middle + 1]
+}
+
+method RightLoopBody(arr: array<int>, a: array<int>, i: nat, middle: nat) 
+	requires a.Length >= 2 && middle == (a.Length - 1) / 2 && i < arr.Length == a.Length - (middle + 1) && isValidIndex(a, middle) 
+	requires Inv2(a, arr, middle, i)
+	ensures Inv2(a, arr, middle, i+1)
+	modifies arr
+{
+	// Assignment
+	LemmaArrIRight(arr, a, i, middle);
+	arr[i] := a[i + middle + 1];
+} 
+
+lemma LemmaArrIRight(arr: array<int>, a: array<int>, i: nat, middle: nat)
+	requires a.Length >= 2 && middle == (a.Length - 1) / 2 && i < arr.Length == a.Length - (middle + 1) && isValidIndex(a, middle) 
+	requires Inv2(a, arr, middle, i)
+	ensures arr[..i] + [a[i + middle + 1]] == a[middle+1 .. (i + middle + 2)]
+{}
+
+method {:verify false} MergeSort3(a: array<int>, left: array<int>, right: array<int>, middle: nat, i1: nat, i2: nat) returns (b: array<int>)
+	requires isLeftArr(a, left, middle, i1) && isRightArr(a, right, middle, i2)
+	requires left.Length + right.Length == a.Length
+	ensures b.Length == a.Length && Sorted(b) && multiset(a[..]) == multiset(b[..])
+	decreases a.Length, 1
+{
+	// Sequential Composition
+	var sortedL, sortedR := MergeSort3a(a, left, right, middle, i1, i2);
+	b := MergeSort3b(a, left, right, sortedL, sortedR, middle);
+}
+
+method MergeSort3a(a: array<int>, left: array<int>, right: array<int>, middle: nat, i1: nat, i2: nat) returns (sortedL: array<int>, sortedR: array<int>)
+	requires isLeftArr(a, left, middle, i1) && isRightArr(a, right, middle, i2)
+	requires left.Length + right.Length == a.Length
+	ensures isSorted(left, sortedL) && isSorted(right, sortedR)
+	ensures sortedL.Length + sortedR.Length == a.Length
+	decreases a.Length, 0
+{
+	// Sequential Composition
+	sortedL := MergeSort(left);
+	sortedR := MergeSort(right);
 }
 
 predicate isSorted(origin: array<int>, sortedArr: array<int>)
@@ -31,232 +218,96 @@ predicate isSorted(origin: array<int>, sortedArr: array<int>)
 	sortedArr.Length == origin.Length && Sorted(sortedArr) && multiset(origin[..]) == multiset(sortedArr[..])
 }
 
-method {:verify false} MergeSort(a: array<int>) returns (b: array<int>)
-	ensures b.Length == a.Length && Sorted(b) && multiset(a[..]) == multiset(b[..])
-	decreases a.Length
-	{
-		if (a.Length < 2) {
-			b := Assign1(a);
-		} else {
-			b := MergeSort1(a);
-		}
-	}
-
-method {:verify false} Assign1 (a: array<int>) returns (b: array<int>)
-	requires a.Length < 2
-	ensures b.Length == a.Length && Sorted(b) && multiset(a[..]) == multiset(b[..])
-{
-	LemmaS1(a);
-	b := a;
-}
-
-lemma LemmaS1 (a: array<int>) 
-	requires a.Length < 2
-	ensures a.Length == a.Length && Sorted(a) && multiset(a[..]) == multiset(a[..])
-
-{}
-
-method {:verify false} MergeSort1 (a: array<int>) returns (b: array<int>)
-	requires a.Length >= 2
-	ensures b.Length == a.Length && Sorted(b) && multiset(a[..]) == multiset(b[..])
-{
-	// Sequential Composition
-	var middle := AssignMiddle(a);
-	b := MergeSort2(a, middle);
-
-}
-
-method {:verify false} MergeSort2 (a: array<int>, middle: nat) returns (b: array<int>) 
-	requires a.Length >= 2
-	requires middle == (a.Length - 1) / 2 && 0 < middle < a.Length
-	ensures b.Length == a.Length && Sorted(b) && multiset(a[..]) == multiset(b[..])
-{
-	// Sequential Composition
-	var left, right := Assign3Split(a, middle);
-	b := MergeSort3(a, left, right, middle);
-}
-
-method {:verify false} AssignMiddle (a: array<int>) returns (m: nat) 
-	requires a.Length >= 2
-	ensures m == (a.Length - 1) / 2 && 0 <= m < a.Length
-{
-	LemmaS2(a);
-	m := (a.Length - 1) / 2;
-}
-
-lemma LemmaS2 (a: array<int>) 
-	requires a.Length >= 2
-	ensures (a.Length - 1) / 2 == (a.Length - 1) / 2 && 0 <= (a.Length - 1) / 2 < a.Length 
-{}
-
-
-method {:verify false} Assign3Split (a: array<int>, middle: nat) returns (left: array<int>, right: array<int>)
-	requires a.Length >= 2 && middle == (a.Length - 1) / 2 && 0 <= middle < a.Length
-	ensures isLeftArr(a, left, middle)
-	ensures isRightArr(a, right, middle)
-{
-	left := Assign3Left(a, middle);
-	right :=  Assign3Right(a, middle);
-}
-
-method {:verify false} Assign3Left(a: array<int>, middle: nat) returns (arr: array<int>) 
-	requires a.Length >= 2 && middle == (a.Length - 1) / 2 && 0 <= middle < a.Length
-	ensures isLeftArr(a, arr, middle) && arr.Length < a.Length
-{
-	var i := 0;
-	arr := new int[middle+1];
-	while (i < middle + 1) 
-		decreases middle + 1 - i
-		invariant forall j :: 0 <= j < i < arr.Length  ==> arr[j] == a[j];
-	{
-		// I is increasing by one
-		// arr[i] = a[i]
-		LeftLoopBody(arr, a, i, middle); //following assignment
-		i := i + 1;
-	}
-} 
-
-method {:verify true} LeftLoopBody(arr: array<int>, a: array<int>, i: nat, middle: nat) 
-	requires a.Length >= 2 && middle == (a.Length - 1) / 2 && middle >= 0 // Pre
-	requires arr.Length == middle + 1
-	requires i < middle + 1 && forall j :: 0 <= j < i < arr.Length ==> arr[j] == a[j]
-	ensures forall j :: 0 <= j < i + 1  < arr.Length ==> arr[j] == a[j] // post cond of following assignment
-	modifies arr
-{
-	LemmaArrI(arr, a, i, middle, a[i]);
-	arr[i] := a[i];
-} 
-
-lemma  LemmaArrI(arr: array<int>, a: array<int>, i: nat, middle: nat, ai: int)
-	requires a.Length >= 2 && middle == (a.Length - 1) / 2 && middle >= 0 // Pre
-	requires arr.Length == middle + 1 >= 1
-	requires i < middle + 1 && forall j :: 0 <= j < i < arr.Length ==> arr[j] == a[j]
-	requires ai == a[i]
-	ensures arr[..i] + [ai] == a[..i+1]
-{}
-method {:verify true}  Assign3Right(a: array<int>, middle: nat) returns (arr: array<int>) 
-	requires a.Length >= 2 && middle == (a.Length - 1) / 2 && 0 < middle < a.Length && arr.Length < a.Length
-	// ensures isRightArr(a, arr, middle)
-	ensures forall i :: 0 <= i < arr.Length < a.Length ==> arr[i] == a[i + middle + 1]
-{
-	var i := 0;
-	arr := new int[a.Length - (middle + 1)];
-	while (i < arr.Length)
-		decreases a.Length - (i + middle + 1)
-		invariant forall j :: 0 <= j < i < arr.Length ==> arr[j] == a[j + middle + 1]
-	{
-		// I is increasing by one
-		// arr[i] = a[i]
-		RightLoopBody(arr, a, i, middle); // following assignment
-		i := i + 1;
-	}
-	// assert forall j :: 0 <= j < arr.Length  ==> arr[j] == a[j + (middle + 1)];
-} 
-
-method {:verify true}  RightLoopBody(arr: array<int>, a: array<int>, i: nat, middle: nat) 
-	requires a.Length >= 2 && middle == (a.Length - 1) / 2 && 0 <= middle < a.Length // Pre
-	requires 0 <= i < a.Length - (middle + 1) // Guard
-	requires forall j :: 0 <= j < i < arr.Length ==> arr[j] == a[j + middle + 1] // Inv
-	requires arr.Length == a.Length - (middle + 1)
-
-	ensures forall j :: 0 <= j < i + 1 < arr.Length ==> arr[j] == a[j + middle + 1] // post cond of following assignment
-	modifies arr
-{
-	assert forall j :: 0 <= j < i  ==> arr[j] == a[j + (middle + 1)];
-	LemmaArrIRight(arr, a, i, middle, a[i + middle + 1]);
-	arr[i] := a[i + middle + 1];
-} 
-
-lemma LemmaArrIRight(arr: array<int>, a: array<int>, i: nat, middle: nat, ai: int)
-	requires a.Length >= 2 && middle == (a.Length - 1) / 2 && 0 <= middle < a.Length // Pre
-	requires 0 <= i < a.Length - (middle + 1) // Guard
-	requires ai == a[i + middle + 1] && arr.Length == a.Length - (middle + 1)
-	requires forall j :: 0 <= j < i < arr.Length ==> arr[j] == a[j + middle + 1] // Inv
-	ensures arr[..i] + [ai] == a[middle+1 .. (i + middle + 2)]
-{}
-
-method {:verify true}  MergeSort3(a: array<int>, left: array<int>, right: array<int>, middle: nat) returns(b: array<int>)
-	requires isLeftArr(a, left, middle) && isRightArr(a, right, middle)
-	ensures b.Length == a.Length && Sorted(b) && multiset(a[..]) == multiset(b[..])
-{
-	//Sequantion composition
-	var sortedL, sortedR := MergeSort3a(a, left, right, middle);
-	b := MergeSort3b(a, left, right,sortedL, sortedR, middle);
-}
-
-method {:verify true}  MergeSort3a(a: array<int>, left: array<int>, right: array<int>, middle: nat) returns(sortedL: array<int>, sortedR: array<int>)
-	requires isLeftArr(a, left, middle) && isRightArr(a, right, middle)
-	ensures isSorted(left, sortedL) && isSorted(right, sortedR)
-	
-{
-	//Sequantion composition
-	sortedL := MergeSort(left);
-	sortedR := MergeSort(right);
-}
-
 method {:verify true}  MergeSort3b(a: array<int>, left: array<int>, right: array<int>,sortedL: array<int>, sortedR: array<int>, middle: nat) returns(b: array<int>)
-	requires isLeftArr(a, left, middle) && isRightArr(a, right, middle)
 	requires isSorted(left, sortedL) && isSorted(right, sortedR)
-	{
-		b := new int[a.Length];
-		Merge(b, sortedL, sortedR);
-	}
+	requires sortedL.Length + sortedR.Length == a.Length
+	ensures b.Length == a.Length && Sorted(b) && multiset(b[..]) == multiset(sortedR[..])+multiset(sortedL[..])
+{
+	b := new int[a.Length];
+	Merge(b, sortedL, sortedR);
+}
 
-
-method {:verify true}  Merge(b: array<int>, c: array<int>, d: array<int>)
+method Merge(b: array<int>, c: array<int>, d: array<int>)
 	requires b != c && b != d && b.Length == c.Length + d.Length
 	requires Sorted(c) && Sorted(d)
-	ensures Sorted(b) && multiset(b[..]) == multiset(c[..])+multiset(d[..])
+	ensures Sorted(b) && multiset(b[..]) == multiset(c[..]) + multiset(d[..])
 	modifies b
-	{
-		var k,l,r := 0,0,0;
-		k,l,r := MergeWhileLoop(b, c, d, k, l, r);
-		assert ((l == c.Length && r < d.Length) || (l < c.Length && r == d.Length));
-		MergeRest(b, c, d, k, l, r);
-	}
-
-predicate CrossSorted(b: array<int>, c: array<int>, d: array<int>, k: nat, l: nat, r: nat) 
-	reads b, c, d
 {
-	forall i, n, m :: (0 <= i < k < b.Length && l <= n < c.Length && r <= m < d.Length) ==> b[i] <= c[n] && b[i] <= d[m] // Sorted(b[.. k])
+	var k,l,r := 0,0,0;
+	// Seq Composition
+	k, l, r := MergeWhileLoop(b, c, d, k, l, r);
+	k, l, r := MergeRest(b, c, d, k, l, r);
 }
+
+method {:verify true} MergeWhileLoop(b: array<int>, c: array<int>, d: array<int>, k0: nat, l0: nat, r0: nat) returns(k: nat, l: nat, r: nat)
+	requires b != c && b != d && b.Length == c.Length + d.Length
+	requires Sorted(c) && Sorted(d) 
+	requires k0 == 0 && l0 == 0 && r0 == 0
+	ensures MergeInv(b,c,d,k,l,r) && !Guard1(b,c,d,k,l,r) && (l == c.Length || r == d.Length)
+	modifies b
+{
+	k, l, r := k0, l0, r0;
+	// Iteration
+	while (Guard1(b,c,d,k,l,r))
+		decreases b.Length - k
+		invariant MergeInv(b,c,d,k,l,r)
+	{
+		ghost var V0 := b.Length - k;
+		// Following Assignment k
+		k,l,r := MergeLoopBody(b, c, d, k, l, r);
+		assert 0 <= b.Length - k - 1 < V0;
+		k := k + 1;
+		assert 0 <= b.Length - k < V0;
+	}
+}
+
+predicate method Guard1(b: array<int>, c: array<int>, d: array<int>, k: nat, l: nat, r: nat)
+	requires 0 <= k && 0 <= l && 0 <= r
+{
+	l != c.Length && r != d.Length && k < b.Length
+}
+
 predicate MergeInv(b: array<int>, c: array<int>, d: array<int>, k: nat, l: nat, r: nat) 
 	reads b, c, d
 {
 	 0 <= k <= b.Length && 0 <= l <= c.Length && 0 <= r <= d.Length &&  k == l + r && 
-	 multiset(b[..k]) == multiset(c[..l] + d[..r]) && CrossSorted(b,c,d,k,l,r) &&
-	 forall i,j :: 0 <= j < i < k ==> b[j] <= b[i] // Sorted(b[.. k])
+	 multiset(b[..k]) == multiset(c[..l] + d[..r]) && CrossSorted2(b,c,d,k,l,r) &&
+	(forall i,j :: 0 <= j < i < k ==> b[j] <= b[i]) // Sorted(b[.. k])
 }
 
-predicate areValidIndices (b: array<int>, c: array<int>, d: array<int>, k: int, l: int, r: int) 
+predicate CrossSorted(b: array<int>, c: array<int>, d: array<int>, k: nat, l: nat, r: nat) 
+	reads b, c, d
 {
-	0 <= k < b.Length && 0 <= l < c.Length && 0 <= r < d.Length 	
+	forall i, n, m :: 0 <= i < k < b.Length && l <= n < c.Length && r <= m < d.Length ==> b[i] <= c[n] && b[i] <= d[m]
 }
-method {:verify false}  MergeWhileLoop(b: array<int>, c: array<int>, d: array<int>, k0: nat, l0: nat, r0: nat) returns(k: nat, l: nat, r: nat)
+
+predicate CrossSorted2(b: array<int>, c: array<int>, d: array<int>, k: nat, l: nat, r: nat) 
+	reads b, c, d
+{
+	(forall i,j :: 0 <= i < k < b.Length && l <= j < c.Length ==> b[i] <= c[j]) &&
+	(forall i,j :: 0 <= i < k < b.Length && r <= j < d.Length ==> b[i] <= d[j])
+}
+
+predicate CrossSorted3(b: array<int>, c: array<int>, d: array<int>, k: nat, l: nat, r: nat) 
+	reads b, c, d
+{
+	(forall i,j :: 0 <= i < k < b.Length && r <= j < d.Length ==> b[i] <= d[j])
+}
+
+predicate CrossSorted4(b: array<int>, c: array<int>, d: array<int>, k: nat, l: nat, r: nat) 
+	reads b, c, d
+{
+	(forall i,j :: 0 <= i < k < b.Length && l <= j < c.Length ==> b[i] <= c[j])
+}
+
+method MergeLoopBody(b: array<int>, c: array<int>, d: array<int>, k0: nat, l0: nat, r0: nat) returns(k: nat, l: nat, r: nat)
 	requires b != c && b != d && b.Length == c.Length + d.Length
 	requires Sorted(c) && Sorted(d) 
-	requires k0 == 0 && l0 == 0 && r0 == 0
-	ensures MergeInv(b,c,d,k,l,r) 
-	ensures (l == c.Length && r < d.Length) || (l < c.Length && r == d.Length)
+	requires MergeInv(b,c,d,k0,l0,r0) && Guard1(b,c,d,k0,l0,r0)  // Inv & Guard
+	ensures MergeInv(b,c,d,k+1,l,r) && k + 1 == (l + r) > (l0 + r0)
 	modifies b
 {
-	k, l, r := k0, l0, r0;
-	while (r < d.Length && l < c.Length && k < b.Length)
-		decreases b.Length - k
-		invariant MergeInv(b,c,d,k,l,r)
-	{
-		// Following Assignment k
-		k,l,r := MergeLoopBody(b, c, d, k, l, r);
-		k := k + 1;
-	}
-}
-
-method {:verify false} MergeLoopBody(b: array<int>, c: array<int>, d: array<int>, k0: nat, l0: nat, r0: nat) returns(k: nat, l: nat, r: nat)
-	requires b != c && b != d && b.Length == c.Length + d.Length
-	requires Sorted(c) && Sorted(d) 
-	requires MergeInv(b,c,d,k0,l0,r0) && k0 < b.Length && l0 < c.Length && r0 < d.Length  // Inv & Guard
-	ensures MergeInv(b,c,d,k+1,l,r) && 0 <= l <= c.Length && r0 + l0 < r + l
-{
+	// Alternation
 	k, l, r := k0, l0, r0;
 	if (c[l] <= d[r]) {
 		// Following Assignment l
@@ -269,154 +320,196 @@ method {:verify false} MergeLoopBody(b: array<int>, c: array<int>, d: array<int>
 	}
 }
 
-method {:verify true}  MergeLoopBody1(b: array<int>, c: array<int>, d: array<int>, k0: nat, l0: nat, r0: nat) 
+method MergeLoopBody1(b: array<int>, c: array<int>, d: array<int>, k0: nat, l0: nat, r0: nat) 
 	requires b != c && b != d && b.Length == c.Length + d.Length
 	requires Sorted(c) && Sorted(d) 
-	requires MergeInv(b,c,d,k0,l0,r0) && k0 < b.Length && l0 < c.Length && r0 < d.Length  // Inv & Guard
+	requires MergeInv(b,c,d,k0,l0,r0) && Guard1(b,c,d,k0,l0,r0)
 	requires c[l0] <= d[r0] // If Test
 	ensures MergeInv(b,c,d,k0+1,l0+1,r0)
 	modifies b
 {
-	// Following assignment k0+1
-	LemmaLB1(b,c,d,k0+1,l0+1,r0);
+	// Assignment 
+	LemmaLB1(b,c,d,k0,l0,r0);
 	b[k0] := c[l0];
 }
 
 lemma LemmaLB1(b: array<int>, c: array<int>, d: array<int>, k: nat, l: nat, r: nat)
 	requires b != c && b != d && b.Length == c.Length + d.Length
 	requires Sorted(c) && Sorted(d) 
-	requires areValidIndices(b,c,d,k-1,l-1,r) && MergeInv(b,c,d,k-1,l-1,r) 
-	requires c[l-1] <= d[r] // If Test
-	// Modify MergeInv
+	requires MergeInv(b,c,d,k,l,r) && Guard1(b,c,d,k,l,r)
+	requires c[l] <= d[r] // If Test
+
+	// Modified MergeInv simulates b[..k] + c[l]
 	ensures 0 <= k <= b.Length && 0 <= l <= c.Length && 0 <= r <= d.Length &&  k == l + r && 
-	 multiset(b[..k-1] + [c[l-1]]) == multiset(c[..l] + d[..r]) && 
-	 forall i, n, m :: (0 <= i < k - 1 < b.Length && l <= n < c.Length && r <= m < d.Length) ==> b[i] <= c[n] && b[i] <= d[m] && c[l-1] <= d[m] // Sorted(b[.. k])  
-	ensures forall i,j :: 0 <= j < i < k - 1 ==> b[j] <= b[i] && b[j] <= c[l-1] // Sorted(b[.. k])
+	multiset(b[..k] + [c[l]]) == multiset(c[..l+1] + d[..r]) && 
+	forall i, n, m :: 0 <= i < k < b.Length && l + 1 <= n < c.Length && r <= m < d.Length ==> 
+	b[i] <= c[n] && b[i] <= d[m] && c[l] <= d[m] && c[l] <= c[n] // CrossSorted(b[..k] + c[l],c,d,k+1,l+1,r)
+	ensures forall i,j :: 0 <= j < i < k ==> b[j] <= b[i] && b[j] <= c[l] // Sorted(b[.. k+1])
 {}
 
-method {:verify true}  MergeLoopBody2(b: array<int>, c: array<int>, d: array<int>, k0: nat, l0: nat, r0: nat) 
+method MergeLoopBody2(b: array<int>, c: array<int>, d: array<int>, k0: nat, l0: nat, r0: nat) 
 	requires b != c && b != d && b.Length == c.Length + d.Length
 	requires Sorted(c) && Sorted(d) 
-	requires MergeInv(b,c,d,k0,l0,r0) && k0 < b.Length && l0 < c.Length && r0 < d.Length  // Inv & Guard
+	requires MergeInv(b,c,d,k0,l0,r0) && Guard1(b,c,d,k0,l0,r0)
 	requires c[l0] > d[r0] // !If Test
 	ensures MergeInv(b,c,d,k0+1,l0,r0+1)
 	modifies b
 {
-	// Following assignment k0+1
-	LemmaLB2(b,c,d,k0+1,l0,r0+1);
+	// Assignment
+	LemmaLB2(b,c,d,k0,l0,r0);
 	b[k0] := d[r0];
 }
-
 lemma LemmaLB2(b: array<int>, c: array<int>, d: array<int>, k: nat, l: nat, r: nat)
 	requires b != c && b != d && b.Length == c.Length + d.Length
 	requires Sorted(c) && Sorted(d) 
-	requires areValidIndices(b,c,d,k-1,l,r-1) && MergeInv(b,c,d,k-1,l,r-1) 
-	requires c[l] > d[r-1] // !If Test
-	// Modify MergeInv
+	requires MergeInv(b,c,d,k,l,r) && Guard1(b,c,d,k,l,r)
+	requires c[l] > d[r] // !If Test
+
+	// Modified MergeInv simulates b[..k] + d[r]
 	ensures 0 <= k <= b.Length && 0 <= l <= c.Length && 0 <= r <= d.Length &&  k == l + r && 
-	 multiset(b[..k-1] + [d[r-1]]) == multiset(c[..l] + d[..r]) && 
-	 forall i, n, m :: (0 <= i < k - 1 < b.Length && l <= n < c.Length && r <= m < d.Length) ==> b[i] <= c[n] && b[i] <= d[m] && d[r-1] <= c[n] // Sorted(b[.. k])  
-	ensures forall i,j :: 0 <= j < i < k - 1 ==> b[j] <= b[i] && b[j] <= d[r-1] // Sorted(b[.. k])
+	 multiset(b[..k] + [d[r]]) == multiset(c[..l] + d[..r+1]) && 
+	 forall i, n, m :: (0 <= i < k < b.Length && l <= n < c.Length && r + 1 <= m < d.Length) ==> 
+	 b[i] <= c[n] && b[i] <= d[m] && d[r] <= c[n] && d[r] <= d[m] // CrossSorted(b[..k] + c[l],c,d,k+1,l,r+1)  
+	ensures forall i,j :: 0 <= j < i < k ==> b[j] <= b[i] && b[j] <= d[r] // Sorted(b[.. k])
 {}
 
-method {:verify true}  MergeRest(b: array<int>, c: array<int>, d: array<int>, k: nat, l: nat, r: nat)
+method {:verify false}  MergeRest(b: array<int>, c: array<int>, d: array<int>, k0: nat, l0: nat, r0: nat) returns (k: nat, l: nat, r: nat)
 	requires b != c && b != d && b.Length == c.Length + d.Length
 	requires Sorted(c) && Sorted(d)
-	requires MergeInv(b,c,d,k,l,r) && ((l == c.Length && r < d.Length) || (l < c.Length && r == d.Length))
-	ensures Sorted(b) && multiset(b[..]) == multiset(c[..])+multiset(d[..])
+	requires MergeInv(b,c,d,k0,l0,r0) && !Guard1(b,c,d,k0,l0,r0)  
+	ensures Sorted(b) && multiset(b[..]) == multiset(c[..]) + multiset(d[..]) 
 	modifies b 
 {
-	if (l == c.Length) {
-		MergeRest1(b,c,d,k,l,r);
-	} else {
-		MergeRest2(b,c,d,k,l,r);
-	}
+		k, l, r := k0, l0, r0;
+		// Alternation
+		if (l0 == c.Length && r0 != d.Length) {
+			k, l, r := MergeRest1(b,c,d,k,l,r);
+			NiceLemma(b,c,d,k,l,r);
+		} else if (r0 == d.Length && l0 != c.Length) {
+			k, l, r := MergeRest2(b,c,d,k,l,r);
+			NiceLemma(b,c,d,k,l,r);
+		} else {
+			NiceLemma(b,c,d,k,l,r);
+		}
 }
 
-predicate MergeRestInv(b: array<int>, c: array<int>, d: array<int>, k: nat, l: nat, r: nat) 
+method MergeRest1(b: array<int>, c: array<int>, d: array<int>, k0: nat, l0: nat, r0: nat) returns (k: nat, l: nat, r: nat)
+	requires b != c && b != d && b.Length == c.Length + d.Length
+	requires Sorted(c) && Sorted(d)
+	requires l0 == c.Length
+	requires MergeInv(b,c,d,k0,l0,r0) && !Guard1(b,c,d,k0,l0,r0)
+	ensures MergeRestInv1(b,c,d,k,l,r) && !Guard2(b,c,d,k,l,r) && r == d.Length && l == c.Length
+	modifies b
+{
+	k, l, r := k0, l0, r0;
+	// Iteration
+	while (Guard2(b,c,d,k,l,r)) 
+		decreases b.Length - k
+		invariant MergeRestInv1(b,c,d,k,l,r) 
+	{
+		ghost var V0 := b.Length - k;
+		// Following Assignment
+		assert 0 <= b.Length - k - 1 < V0;
+		MergeRestBody1(b,c,d,k,l,r);
+		k, r := k + 1, r + 1;
+		assert 0 <= b.Length - k < V0;
+	}
+}
+predicate MergeRestInv1(b: array<int>, c: array<int>, d: array<int>, k: nat, l: nat, r: nat) 
 	reads b, c, d
 {
 	 0 <= k <= b.Length && 0 <= l <= c.Length && 0 <= r <= d.Length &&  k == l + r && 
-	 multiset(b[..k]) == multiset(c[..l] + d[..r]) && 
-	 forall i,j :: 0 <= j < i < k ==> b[j] <= b[i] // Sorted(b[.. k])
+	 multiset(b[..k]) == multiset(c[..l] + d[..r]) && CrossSorted3(b,c,d,k,l,r) &&
+	(forall i,j :: 0 <= j < i < k ==> b[j] <= b[i]) // Sorted(b[.. k])
+}
+predicate MergeRestInv2(b: array<int>, c: array<int>, d: array<int>, k: nat, l: nat, r: nat) 
+	reads b, c, d
+{
+	 0 <= k <= b.Length && 0 <= l <= c.Length && 0 <= r <= d.Length &&  k == l + r && 
+	 multiset(b[..k]) == multiset(c[..l] + d[..r]) && CrossSorted4(b,c,d,k,l,r) &&
+	(forall i,j :: 0 <= j < i < k ==> b[j] <= b[i]) // Sorted(b[.. k])
 }
 
-predicate CrossSortedRest1(b: array<int>, arr: array<int>, k: nat, index: nat) 
-	reads b, arr
-{
-	forall i, n :: (0 <= i < k < b.Length && index <= n < arr.Length ) ==> b[i] <= arr[n] 
-}
-method {:verify true}  MergeRest1(b: array<int>, c: array<int>, d: array<int>, k: nat, l: nat, r: nat)
+method {:verify true}  MergeRestBody1(b: array<int>, c: array<int>, d: array<int>, k: nat, l: nat, r: nat) 
 	requires b != c && b != d && b.Length == c.Length + d.Length
 	requires Sorted(c) && Sorted(d)
-	requires MergeInv(b,c,d,k,l,r)
-	requires ((l == c.Length && r < d.Length) || (l < c.Length && r == d.Length)) && l == c.Length//r < d.Length // Guard
-	ensures Sorted(b) && multiset(b[..]) == multiset(c[..])+multiset(d[..]) 
+	requires MergeRestInv1(b,c,d,k,l,r) && Guard2(b,c,d,k,l,r)
+	ensures MergeRestInv1(b,c,d,k+1,l,r+1)
 	modifies b
 {
-	var r1: nat, k1: nat := r, k;
-	while (k1 < b.Length && r1 < d.Length) 
-		decreases b.Length - k1
-		invariant MergeRestInv(b,c,d,k1,l,r1) 
+	// Assignment
+	b[k] := d[r];
+}
+
+method MergeRest2(b: array<int>, c: array<int>, d: array<int>, k0: nat, l0: nat, r0: nat) returns (k: nat, l: nat ,r: nat)
+	requires b != c && b != d && b.Length == c.Length + d.Length
+	requires Sorted(c) && Sorted(d)
+	requires l0 != c.Length 
+	requires MergeInv(b,c,d,k0,l0,r0) && !Guard1(b,c,d,k0,l0,r0)
+	ensures MergeRestInv2(b,c,d,k,l,r) && !Guard3(b,c,d,k,l,r) && l == c.Length && r == d.Length
+	modifies b
+{
+	k, l, r := k0, l0, r0;
+	// Iteration
+	while (Guard3(b,c,d,k,l,r)) 
+		decreases b.Length - k
+		invariant MergeRestInv2(b,c,d,k,l,r) 
 	{
-
-
-		assert r1 < d.Length;
-		b[k1] := d[r1];
-		r1 := r1 + 1;
-		k1 := k1 + 1;
-
-
-		assert 0 <= k1 <= b.Length;
-		assert 0 <= l <= c.Length;
-		assert 0 <= r1 <= d.Length;
-		assert  k1 == l + r1;
-	 	assert multiset(b[..k1]) == multiset(c[..l] + d[..r1]);
-	 	assert forall i,j :: 0 <= j < i < k1 < b.Length ==> b[j] <= b[i]; // Sorted(b[.. k])
+		ghost var V0 := b.Length - k;
+		// Following Assignment
+		MergeRestBody2(b,c,d,k,l,r);
+		assert 0 <= b.Length - k - 1 < V0;
+		k, l := k + 1, l + 1;		
+		assert 0 <= b.Length - k < V0;
 	}
 }
 
-method {:verify true}  MergeRest2(b: array<int>, c: array<int>, d: array<int>, k: nat, l: nat, r: nat)
+method {:verify true}  MergeRestBody2(b: array<int>, c: array<int>, d: array<int>, k: nat, l: nat, r: nat) 
 	requires b != c && b != d && b.Length == c.Length + d.Length
 	requires Sorted(c) && Sorted(d)
-	requires MergeInv(b,c,d,k,l,r)
-	requires l < c.Length // Guard
-	ensures Sorted(b) && multiset(b[..]) == multiset(c[..])+multiset(d[..]) 
+	requires MergeRestInv2(b,c,d,k,l,r) && Guard3(b,c,d,k,l,r)
+	ensures MergeRestInv2(b,c,d,k+1,l+1,r)
 	modifies b
 {
-	var l1: nat, k1: nat := l, k;
-	assert l1 < d.Length;
-	while (k1 < b.Length && l1 < c.Length) 
-		decreases b.Length - k1
-		invariant MergeRestInv(b,c,d,k1,l1,r) 
-	{
-		b[k1] := c[l1];
-		l1 := l1 + 1;
-		k1 := k1 + 1;
-		// assert 0 <= k1 <= b.Length;
-		// assert 0 <= l <= c.Length;
-		// assert 0 <= r1 <= d.Length;
-		// assert  k1 == l + r1;
-	 	// assert multiset(b[..k1]) == multiset(c[..l] + d[..r1]);
-	}
+	// Assignment
+	b[k] := c[l];
+}
+
+lemma NiceLemma(b: array<int>, c: array<int>, d: array<int>, k: nat, l: nat, r: nat)
+	requires b != c && b != d && b.Length == c.Length + d.Length
+	requires Sorted(c) && Sorted(d)
+	requires l == c.Length && r == d.Length
+	requires (MergeRestInv1(b,c,d,k,l,r) && !Guard2(b,c,d,k,l,r) && r == d.Length && l == c.Length) || 
+			 (MergeRestInv2(b,c,d,k,l,r) && !Guard3(b,c,d,k,l,r) && r == d.Length && l == c.Length)
+	requires multiset(b[..(b.Length)]) == multiset(c[..(c.Length)])+multiset(d[..(d.Length)])
+	requires multiset(b[..(b.Length)]) == multiset(b[..])
+	requires multiset(c[..(c.Length)]) == multiset(c[..])
+	requires multiset(d[..(d.Length)]) == multiset(d[..])
+	ensures l == c.Length && r == d.Length && k == b.Length
+	ensures Sorted(b) && multiset(b[..k]) == multiset(c[..])+multiset(d[..])
+{
+	assert l == c.Length && r == d.Length && b.Length == c.Length + d.Length && k == l + r ==> k == b.Length;
+}
+
+predicate method Guard2(b: array<int>, c: array<int>, d: array<int>, k: nat, l: nat, r: nat) 
+{
+	k != b.Length && r != d.Length
+}
+
+predicate method Guard3(b: array<int>, c: array<int>, d: array<int>, k: nat, l: nat, r: nat) 
+{
+	k != b.Length && l != c.Length
 }
 
 method Main() {
-	var a := new int[6];
-	a[0] := 10;
-	a[1] := 39;
-	a[2] := 1;
-	a[3] := 0;
-	a[4] := -1;
-	a[5] := 2;
+	var a := new int[3];
+	a[0], a[1], a[2] := 4, 8, 6;
 	var q0 := a[..];
-	// assert q0 == [4,8,6];
+	assert q0 == [4,8,6];
 	a := MergeSort(a);
-	// assert a.Length == |q0| && multiset(a[..]) == multiset(q0);
+	assert a.Length == |q0| && multiset(a[..]) == multiset(q0);
 	print "the sorted version of [4, 8, 6] is ";
 	print a[..];
-	// assert Sorted(a);
-	// assert a[..] == [4,6,8];
+	assert Sorted(a);
+	assert a[..] == [4,6,8];
 }
-
-
